start with soundness proof

thys/MFODL_Monitor_Devel/Type_Soundness.thy
@@ -10,8 +10,8 @@ undef_divide :: "event_data \<Rightarrow> event_data \<Rightarrow> event_data" a
 undef_modulo :: "event_data \<Rightarrow> event_data \<Rightarrow> event_data"  and
 undef_double_of_event_data :: "event_data \<Rightarrow> double" and
 undef_integer_of_event_data :: "event_data \<Rightarrow> integer" and
-undef_less_eq :: "event_data \<Rightarrow> event_data \<Rightarrow> bool"
-
+undef_less_eq :: "event_data \<Rightarrow> event_data \<Rightarrow> bool" and
+undef_eq :: "event_data \<Rightarrow> event_data \<Rightarrow> bool"
 assumes undef_plus_sound:  "\<And>x y. EInt x + EInt y = undef_plus (EInt x) (EInt y)" 
     "\<And> x y . EFloat x + EFloat y = undef_plus (EFloat x) (EFloat y)"
 assumes undef_minus_sound:  "\<And>x y. EInt x - EInt y = undef_minus (EInt x) (EInt y)" 
@@ -23,13 +23,27 @@ assumes undef_times_sound:  "\<And>x y. EInt x * EInt y = undef_times (EInt x) (
 assumes undef_divide_sound:  "\<And>x y. EInt x div EInt y = undef_divide (EInt x) (EInt y)" 
     "\<And> x y . EFloat x div EFloat y = undef_divide (EFloat x) (EFloat y)"
 assumes undef_modulo_sound:  "\<And>x y. EInt x mod EInt y = undef_modulo (EInt x) (EInt y)"  
-(* differs from the rules specified in the document
-added change also to wty_trm*)
+assumes undef_eq_sound: "\<And>x y. EInt x = EInt y \<longleftrightarrow> undef_eq (EInt x) (EInt y)"
+ "\<And>x y. EFloat x = EFloat y \<longleftrightarrow> undef_eq (EFloat x) (EFloat y)"
+ "\<And> x y. EString x = EString y \<longleftrightarrow> undef_eq (EString x) (EString y)"
+
 assumes undef_double_of_event_data_sound: "\<And>x. double_of_event_data (EInt x) = undef_double_of_event_data (EInt x)"
 assumes undef_integer_of_event_data_sound: "\<And>x. integer_of_event_data (EFloat x) = undef_integer_of_event_data (EFloat x)"
 
 assumes undef_less_eq_sound: "\<And>x y. EInt x \<le> EInt y \<longleftrightarrow> undef_less_eq (EInt x) (EInt y)"
+ "\<And>x y. EFloat x \<le> EFloat y \<longleftrightarrow> undef_less_eq (EFloat x) (EFloat y)"
+ "\<And> x y. EString x \<le> EString y \<longleftrightarrow> undef_less_eq (EString x) (EString y)"
+
 begin
+
+definition undef_less :: "event_data \<Rightarrow> event_data \<Rightarrow> bool"  where
+  "undef_less x y \<longleftrightarrow> undef_less_eq x y \<and> \<not> undef_less_eq y x"
+
+definition undef_min :: "event_data \<Rightarrow> event_data \<Rightarrow> event_data" where
+  "undef_min a b = (if undef_less_eq a b then a else b)"
+
+definition undef_max :: "event_data \<Rightarrow> event_data \<Rightarrow> event_data" where
+  "undef_max a b = (if undef_less_eq a b then b else a)"
 
 primrec eval_trm' :: "Formula.env \<Rightarrow> Formula.trm \<Rightarrow> event_data" where
   "eval_trm' v (Formula.Var x) = v ! x"
@@ -43,15 +57,45 @@ primrec eval_trm' :: "Formula.env \<Rightarrow> Formula.trm \<Rightarrow> event_
 | "eval_trm' v (Formula.F2i x) = EInt (undef_integer_of_event_data (eval_trm' v x))"
 | "eval_trm' v (Formula.I2f x) = EFloat (undef_double_of_event_data (eval_trm' v x))"
 
+
+fun eval_agg_op' :: "Formula.agg_op \<Rightarrow> (event_data \<times> enat) set \<Rightarrow> event_data" where
+  "eval_agg_op' (agg_type.Agg_Cnt, y0) M = (case (flatten_multiset M, finite_multiset M) of
+    (_, False) \<Rightarrow> y0
+    |    ([],_) \<Rightarrow> y0
+    | (xs,_) \<Rightarrow> EInt (integer_of_int (length xs)))"
+| "eval_agg_op' (agg_type.Agg_Min, y0) M = (case  (flatten_multiset M, finite_multiset M) of
+    (_, False) \<Rightarrow> y0
+    |    ([],_) \<Rightarrow> y0
+    | (x # xs,_) \<Rightarrow> foldl undef_min x xs)"
+| "eval_agg_op' (agg_type.Agg_Max, y0) M = (case  (flatten_multiset M, finite_multiset M) of
+    (_, False) \<Rightarrow> y0
+    |    ([],_) \<Rightarrow> y0
+    | (x # xs,_) \<Rightarrow> foldl undef_max x xs)"
+| "eval_agg_op' (agg_type.Agg_Sum, y0) M = (case  (flatten_multiset M, finite_multiset M) of
+    (_, False) \<Rightarrow> y0
+    |    ([],_) \<Rightarrow> y0
+    | (x # xs,_) \<Rightarrow> foldl undef_plus x xs)"
+| "eval_agg_op' (agg_type.Agg_Avg, y0) M =(case  (flatten_multiset M, finite_multiset M) of
+    (_, False) \<Rightarrow> y0
+    |    ([],_) \<Rightarrow> y0
+    | (x#xs,_) \<Rightarrow> EFloat ( undef_double_of_event_data (foldl undef_plus x xs) / double_of_int (length (x#xs))))"
+| "eval_agg_op' (agg_type.Agg_Med, y0) M =(case (flatten_multiset M, finite_multiset M) of
+    (_, False) \<Rightarrow> y0
+    |    ([],_) \<Rightarrow> y0
+    | (xs,_) \<Rightarrow> EFloat (let u = length xs;  u' = u div 2 in
+          if even u then
+            (undef_double_of_event_data (xs ! (u'-1)) + undef_double_of_event_data (xs ! u') / double_of_int 2)
+          else undef_double_of_event_data (xs ! u')))"
+
 fun sat' :: "Formula.trace \<Rightarrow> (Formula.name \<rightharpoonup> nat \<Rightarrow> event_data list set) \<Rightarrow> Formula.env \<Rightarrow> nat \<Rightarrow> 't Formula.formula \<Rightarrow> bool" where
   "sat' \<sigma> V v i (Formula.Pred r ts) = (case V r of
        None \<Rightarrow> (r, map (eval_trm' v) ts) \<in> \<Gamma> \<sigma> i
      | Some X \<Rightarrow> map (eval_trm' v) ts \<in> X i)"
 | "sat' \<sigma> V v i (Formula.Let p \<phi> \<psi>) =
     sat' \<sigma> (V(p \<mapsto> \<lambda>i. {v. length v = Formula.nfv \<phi> \<and> sat' \<sigma> V v i \<phi>})) v i \<psi>"
-| "sat' \<sigma> V v i (Formula.Eq t1 t2) = (eval_trm' v t1 = eval_trm' v t2)"
-| "sat' \<sigma> V v i (Formula.Less t1 t2) = (eval_trm' v t1 < eval_trm' v t2)"
-| "sat' \<sigma> V v i (Formula.LessEq t1 t2) = (eval_trm' v t1 \<le> eval_trm' v t2)"
+| "sat' \<sigma> V v i (Formula.Eq t1 t2) = undef_eq (eval_trm' v t1) (eval_trm' v t2)"
+| "sat' \<sigma> V v i (Formula.Less t1 t2) = undef_less (eval_trm' v t1) (eval_trm' v t2)"
+| "sat' \<sigma> V v i (Formula.LessEq t1 t2) = undef_less_eq (eval_trm' v t1) (eval_trm' v t2)"
 | "sat' \<sigma> V v i (Formula.Neg \<phi>) = (\<not> sat' \<sigma> V v i \<phi>)"
 | "sat' \<sigma> V v i (Formula.Or \<phi> \<psi>) = (sat' \<sigma> V v i \<phi> \<or> sat' \<sigma> V v i \<psi>)"
 | "sat' \<sigma> V v i (Formula.And \<phi> \<psi>) = (sat' \<sigma> V v i \<phi> \<and> sat' \<sigma> V v i \<psi>)"
@@ -59,7 +103,7 @@ fun sat' :: "Formula.trace \<Rightarrow> (Formula.name \<rightharpoonup> nat \<R
 | "sat' \<sigma> V v i (Formula.Exists t \<phi>) = (\<exists>z. sat' \<sigma> V (z # v) i \<phi>)"
 | "sat' \<sigma> V v i (Formula.Agg y \<omega> tys f \<phi>) =
     (let M = {(x, ecard Zs) | x Zs. Zs = {zs. length zs = length tys \<and> sat' \<sigma> V (zs @ v) i \<phi> \<and> eval_trm' (zs @ v) f = x} \<and> Zs \<noteq> {}}
-    in (M = {} \<longrightarrow> fv \<phi> \<subseteq> {0..< length tys}) \<and> v ! y = eval_agg_op \<omega> M)"
+    in (M = {} \<longrightarrow> fv \<phi> \<subseteq> {0..< length tys}) \<and> v ! y = eval_agg_op' \<omega> M)"
 | "sat' \<sigma> V v i (Formula.Prev I \<phi>) = (case i of 0 \<Rightarrow> False | Suc j \<Rightarrow> mem I (\<tau> \<sigma> i - \<tau> \<sigma> j) \<and> sat' \<sigma> V v j \<phi>)"
 | "sat' \<sigma> V v i (Formula.Next I \<phi>) = (mem I ((\<tau> \<sigma> (Suc i) - \<tau> \<sigma> i)) \<and> sat' \<sigma> V v (Suc i) \<phi>)"
 | "sat' \<sigma> V v i (Formula.Since \<phi> I \<psi>) = (\<exists>j\<le>i. mem I (\<tau> \<sigma> i - \<tau> \<sigma> j) \<and> sat' \<sigma> V v j \<psi> \<and> (\<forall>k \<in> {j <.. i}. sat' \<sigma> V v k \<phi>))"
@@ -67,6 +111,50 @@ fun sat' :: "Formula.trace \<Rightarrow> (Formula.name \<rightharpoonup> nat \<R
 | "sat' \<sigma> V v i (Formula.MatchP I r) = (\<exists>j\<le>i. mem I (\<tau> \<sigma> i - \<tau> \<sigma> j) \<and> Regex.match (sat' \<sigma> V v) r j i)"
 | "sat' \<sigma> V v i (Formula.MatchF I r) = (\<exists>j\<ge>i. mem I (\<tau> \<sigma> j - \<tau> \<sigma> i) \<and> Regex.match (sat' \<sigma> V v) r i j)"
 
+lemma eval_trm_sound: 
+  assumes "E \<turnstile> f :: t"  "\<forall>y\<in>fv_trm f. ty_of (v ! y) = E y"
+  shows "Formula.eval_trm v f = eval_trm' v f"
+  sorry
+lemma soundness:
+  assumes "S,E \<turnstile> \<phi>"  "\<forall>y\<in>fv \<phi>. ty_of (v ! y) = E y"
+  shows "Formula.sat \<sigma> V v i \<phi> \<longleftrightarrow> sat' \<sigma> V v i \<phi>" 
+ using assms  proof (induction \<phi> arbitrary: v V i S )
+case (Pred x1 x2)
+  then show ?case sorry
+next
+  case (Eq E x1 t x2)
+  from this have fv_x1: " \<forall>y\<in>fv_trm x1. ty_of (v ! y) = E y " by auto
+  from Eq have fv_x2: " \<forall>y\<in>fv_trm x2. ty_of (v ! y) = E y " by auto
+  from Eq fv_x2 show ?case using eval_trm_sound  ty_of_eval_trm  apply (cases t)
+    using value_of_eval_trm[of E x2 v  ] value_of_eval_trm[of E x1 v  ]
+    undef_eq_sound apply auto 
+    by blast+
+
+next
+  case (Less E x1 t x2)
+  sorry
+next
+  case (LessEq E x1 t x2)
+  sorry
+next
+  case (Agg x1 x2 x3 x4 \<phi>)
+  then show ?case sorry
+next
+  find_theorems Regex.pred_regex regex.atms
+  case (MatchF S E x2 x1) 
+  from this have "Ball (regex.atms x2) ( \<lambda>\<phi> . S, E \<turnstile> \<phi> \<and> (\<forall>x. (\<forall>ya\<in>fv \<phi>. ty_of (x ! ya) = E ya) \<longrightarrow> (\<forall>xa xb. Formula.sat \<sigma> xa x xb \<phi> = local.sat' \<sigma> xa x xb \<phi>)))"
+    by (simp add: regex.pred_set)
+  from MatchF have "\<And> \<phi> . \<phi> \<in>  regex.atms x2 \<Longrightarrow> \<forall>ya\<in>fv \<phi>. ty_of (v ! ya) = E ya" apply (auto simp add: regex.pred_set)
+  from this have r: "\<phi> \<in> regex.atms x2 \<Longrightarrow> Formula.sat \<sigma> V5 v5 i5 \<phi> = local.sat' \<sigma> V5 v5 i5 \<phi>" for \<phi> V5 v5 i5
+    using regex.pred_set apply auto sledgehammer sorry
+  then show ?case  using match_cong[OF refl r, where ?r=x2] by auto 
+(*   ?x2a5 \<in> regex.atms x2 \<Longrightarrow> Formula.sat \<sigma> ?V5 ?v5 ?i5 ?x2a5 = local.sat' \<sigma> ?V5 ?v5 ?i5 ?x2a5
+  then show ?case  using match_cong[OF refl MatchF, where ?r=x2 and ?x2a6="\<lambda>i j. j"] by auto *)
+next
+  case (MatchP x1 x2) then show ?case sorry
+  (*then show ?case  using match_cong[OF refl MatchP, where ?r=x2 and ?x2a6="\<lambda>i j. j"] by auto *)
+
+qed (auto split: nat.splits)
 
 end
 end
